\documentclass[12pt]{article}
\usepackage{amsmath}
\usepackage{amssymb}
\begin{document}

\section{
    Exercise 13
}
\subsection{
    Show that $\vec{p}^{\,2} = \Vert \vec{p} \Vert^2$
}

\begin{align*}
•
    &\vec{p}^{\,2} \\
    &= \vec{p} \cdot \vec{p} \\
    &= \cos{0} \times \Vert \vec{p} \Vert \Vert \vec{p} \Vert \\ 
    &= \Vert \vec{p} \Vert ^2
\end{align*}

\subsection{
    Show that $\Vert \vec{p} + \vec{q} \Vert^2 = \Vert \vec{p} \Vert^2 + 2 \vec{p} \cdot \vec{q} + \Vert \vec{q} \Vert^2$
}

\begin{align*}
•
    &\Vert \vec{p} + \vec{q} \Vert^2 \\
    &= (\vec{p} + \vec{q})^2 \\
    &= (\vec{p} + \vec{q}) \cdot (\vec{p} + \vec{q}) \\
    &= \vec{p}^{\,2} + 2 \vec{p} \cdot \vec{q} + \vec{q}^{\,2} \\
    &= \Vert \vec{p} \Vert^2 + 2 \vec{p} \cdot \vec{q} + \Vert \vec{q} \Vert^2
\end{align*}

\subsection{
    Deduce that $\Vert \vec{p} + \vec{q} \Vert \leq \Vert \vec{p} \Vert + \Vert \vec{q} \Vert$
}

\begin{align*}
•
    &\Vert \vec{p} + \vec{q} \Vert^2 - (\vec{p} + \vec{q})^2 \\
    &= \Vert \vec{p} \Vert^2 
     + 2 \vec{p} \cdot \vec{q} 
     + \Vert \vec{q} \Vert^2 
     - \Vert \vec{p} \Vert^2 
     - 2 \Vert \vec{p} \Vert \Vert \vec{q} \Vert 
     - \Vert \vec{q} \Vert^2 \\
    &= 2 \cos{\theta} \Vert \vec{p} \Vert \Vert \vec{q} \Vert 
     - 2 \Vert \vec{p} \Vert \Vert \vec{q} \Vert \\
    &= 2 \Vert \vec{p} \Vert \Vert \vec{q} \Vert (\cos{\theta} - 1) \\
    &\cos{\theta} \leq 1 \\
    \Leftrightarrow &\cos{\theta} - 1 \leq 0 \\
    &2 \Vert \vec{p} \Vert \Vert \vec{q} \Vert \geq 0 \\
    \therefore &2 \Vert \vec{p} \Vert \Vert \vec{q} \Vert (\cos{\theta} - 1) \leq 0 \\
    \Leftrightarrow &\Vert \vec{p} + \vec{q} \Vert^2 \leq (\vec{p} + \vec{q})^2 \\
    &\Vert \vec{p} + \vec{q} \Vert \geq 0 \\
    &\vec{p} + \vec{q} \geq 0\\
    \therefore & \Vert \vec{p} + \vec{q} \Vert \leq \Vert \vec{p} \Vert + \Vert \vec{q} \Vert
\end{align*}

\end{document}